\documentclass{article}
\pagestyle{plain}
\usepackage{amsmath}
\usepackage{amssymb} % We use \therefore from this package
\begin{document}

\title{Assignment 3 - Differential Equations }
\date{\today}
\author{Mohan S Nayaka}
\renewcommand{\arraystretch}{1.5}
\maketitle
Exercises
\\
\\
\textbf{1. }$\mathbf{ (3x^2-y^2) dy - 2xydx = 0}$\\
This is a homogeneous differential equation. Hence, we make the substitution:
\[y=zx\]
Thus,\\
\\
\[\frac{dy}{dx}=z+x\frac{dz}{dx}\]
\\
\\
Substituting in the equation, we get:\\
\[(3x^2-z^2x^2)(z+x\frac{dz}{dx})-2x(zx)=0\]\\
\\
Cancelling $x^2$ throughout,\\
\[(3-z^2)(z+x\frac{dz}{dx})-2zx^2=0\]
\\
\\
Simplifying,
\\
\\
\[z+x\frac{dz}{dx}=\frac{2z}{3-z^2}\]
\\
\\
\[x\frac{dz}{dx}=\frac{2z}{3-z^2}-z\]
\\
\\
\[x\frac{dz}{dx}=\frac{2z-3z+z^3}{3-z^2}\]
\\
\\
\[\frac{dz}{dx}=\frac{1}{x}\frac{2z-3z+z^3}{3-z^2}\]
\\
\\
\begin{equation}
\frac{dx}{x}=\frac{3-z^2}{z(z^2-1)} \label{1}
\end{equation}
\\
We will use partial fractions to express the right-hand-side of \eqref{1} as:
\\\[\frac{A}{z}+\frac{B}{z+1}+\frac{C}{z-1}\]
\\
\\
To obtain A, multiply througout by $z$, and set $z=0$,\\
Thus,\\
\[\frac{3-z^2}{(z-1)(z+1)}=A+\frac{Bz}{z+1}+\frac{Cz}{z-1}\]\\
becomes,\\
\begin{center}
\begin{tabular}{|c|}
\hline
$A=\frac{3}{-1}=-3$\\
\hline
\end{tabular}
\\
\end{center}
To obtain B, multiply througout by $z+1$, and set $z=-1$,\\
Thus,\\
\[\frac{3-z^2}{z(z-1)}=A(z+1)+B+\frac{C(z+1)}{z-1}\]\\
becomes,\\
\[B=\frac{2}{(-1)(-2)}\]\\
\begin{center}
\begin{tabular}{|c|}
\hline
$B=1$\\
\hline
\end{tabular}\\
\end{center}
To obtain C, multiply througout by $z-1$, and set $z=1$,\\
Thus,\\
\[\frac{3-z^2}{z(z+1)}=\frac{A(z-1)}{z}+\frac{B(z-1)}{z+1}+C\]\\
becomes,\\
\[C=\frac{2}{(1)(2)}\]\\
\begin{center}
\begin{tabular}{|c|}
\hline
$C=1$\\
\hline
\end{tabular}\\
\end{center}

Substituting the values of A,B and C in equation \eqref{1}, we get:
\[\frac{dx}{x}=\frac{-3}{z}+\frac{1}{z+1}+\frac{1}{z-1}\]\\
Integrating this equation, we get:\\
\\\[ln(x)=ln(z^{-3})+ln(z+1)+ln(z-1)+C_1\]
\\\[x=C_2ln\left(\frac{(z+1)(z-1)}{z^3}\right)\]

Substituting $z=\frac{y}{x}$, we get:\\
\[x=C_2\frac{x^3}{y^3}\frac{x+y}{x}\frac{y-x}{x}\]
\[y^3=C_2(x+y)(y-x)\]
Thus,\\
\begin{center}
\begin{tabular}{|c|}
\hline
$y^3-C(x+y)(x-y)=0$\\
\hline
\end{tabular}
\end{center}
\textbf{2. }$\mathbf{(x-y)dx - (x+y)dy = 0}$\\
This is a homogeneous differential equation. Hence, we make the substitution:
\[y=zx\]
Thus,\\
\[y=zx \Rightarrow \frac{dy}{dx} = z + x \frac{dz}{dx}\]\\
\[x-zx-(x+zx)\left(z+x\frac{dz}{dx}\right)=0\]\\
\[x-zx-\left(zx+x^2\frac{dz}{dx}-z^2x-zx^2\frac{dz}{dx}\right)=0\]\\
Cancelling x throughout and simplifying,\\
\[1-2z-x\frac{dz}{dx}-z^2-zx\frac{dz}{dx}=0\]
\[1-2z-z^2=x(1+z)\frac{dz}{dx}\]
\[\frac{dx}{x}=\frac{1+z}{1-2z-z^2}\]
\[\frac{dx}{x}=\frac{1}{-2}\left(\frac{-2-2z}{1-2z-z^2}\right)dz\]
Integrating, we get:\\
\[\frac{1}{-2}ln(1-2z-z^2)=ln(x)+C_1\]
\[\frac{1}{-2}ln(1-2z-z^2)=ln(C_2x) \]\\Where $C_2 = ln(C_1)$
\[\left(\frac{1}{1-2z-z^2}\right)=C_3x^2 \]\\Where $C_3 = C_2^2$
Substituting $z=y/x$, we get:\\
\[C_3x^2\left(1-2\frac{y}{x}-\frac{y^2}{x^2}\right)=1\]
With $C_4=\frac{1}{C_3}$, we can simplify to obtain the result:\\
\begin{center}
\begin{tabular}{|c|}
\hline
$x^2-2xy-y^2=C$\\
\hline
\end{tabular}
\end{center}

\textbf{3. }$\mathbf{(1+y^2sin2x)dx - 2ycos^2xdy = 0}$\\
Here, we have M=$1+y^2sinx$ and N=$-2ycos^2x$
Thus,\\
\[\frac{\partial M}{\partial y} = 2ysin2x\]
\[\frac{\partial N}{\partial x} = -2y(2 cosx * (-sin x)) = 2ysin2x\]
Thus, the equation is exact and the solution can be written in the form \begin{equation*}f(x,y)=C\end{equation*} where,
\begin{equation}
\frac{\partial f}{\partial x} = M = 1+y^2sinx \label{Fx}
\end{equation}
\begin{equation}
\frac{\partial f}{\partial y} = N = -2ycos^2x \label{Fy}
\end{equation}
Thus,\\
%\begin{center}
\[\frac{\partial f}{\partial x} = 1 + y^2sin2x\]
%\end{center}
\[\therefore f = x + y^2(-cos2x/2) + g(y)\]
\begin{equation}
\therefore f = x - y^2(cos2x/2) + g(y) \label{getgy}
\end{equation}
\[\therefore \frac{\partial f}{\partial y}=0 + 2y \left(\frac{-cos2x}{2}\right) +g'(y)\]\\
Using \eqref{Fy},
\[-2ycos^2x = -ycos2x + g'(y)\]
\[g'(y) = ycos2x-2ycos^2x\]
\[g'(y) = y (2cos^2x - 1) - 2ycos^2x\]
\[g'(y) = 2ycos^2x -y - 2ycos^2x\]
\[g'(y) = -y\]
\begin{equation}
g(y) = \frac{-y^2}{2} \label{gy}
\end{equation}
Given that the solution to the differential equation is $f = c$,
from equations \eqref{getgy} and \eqref{gy}, we have,\\
\[x-y^2\frac{cos2x}{2} -\frac{y^2}{2}=c\]
\[2x-y^2cos2x-y^2=C\]
\begin{center}
where $C=2*c$
\end{center}
\end{document}